VProg/Instructions.v
@@ -14,7 +14,7 @@ Section Read.
     (IJ : InjPre_Frame_Spec [CTX.mka (SLprop.cell p, d)] ctx {|
       sf_csm  := Vector.cons _ false _ (Vector.nil _) <: Sub.t [_];
       sf_prd  := fun _ => nil;
-      sf_spec := FP.Ret (TF.mk _ d Tuple.tt);
+      sf_spec := FP.Ret (TF.mk0 _ d Tuple.tt);
     |} F).
 
   Program Definition Read : instr CT memdata := {|
@@ -49,7 +49,7 @@ Section Write.
     (IJ : InjPre_Frame_Spec [CTX.mka (SLprop.cell p, d0)] ctx {|
       sf_csm  := Vector.cons _ true _ (Vector.nil _) <: Sub.t [_];
       sf_prd  := fun _ => [Vprop.mk (SLprop.cell p)];
-      sf_spec := FP.Ret (TF.mk (fun _ => [memdata]) tt (d, tt));
+      sf_spec := FP.Ret (TF.mk0 (fun _ => [memdata]) tt (d, tt));
     |} F).
 
   Program Definition Write : instr CT unit := {|
@@ -69,14 +69,329 @@ Section Write.
       Apply PRE.
       SL.normalize; reflexivity.
   Qed.
-End Write.
+End Write .
 
 Local Ltac build_Write :=
   simple refine (Write_SpecI _ _ _ _ _ _);
   [ shelve | (* IJ *) Tac.build_InjPre_Frame ].
 
+Section Loop.
+  Context [CT : CP.context] [A B : Type]
+    (* ALT? like function spec / Assert *)
+    (vinv : A + B -> VpropList.t)
+    (sinv : option (forall x : A + B, Tuple.arrow (VpropList.sel (vinv x)) (fun _ => Prop)))
+    (ini : A + B) (f : A -> instr CT (A + B)).
+
+  Fixpoint split_sub_of_ctx1 (vs : VpropList.t) (add : CTX.t) {struct vs}:
+    forall (sl : VpropList.sel_t (vs ++ VpropList.of_ctx add))
+           (sb : Sub.t (VpropList.inst (vs ++ VpropList.of_ctx add) sl)),
+    CTX.t * Sub.t add.
+  Proof.
+    case vs as [|v vs]; cbn.
+    - exact (fun sl sb => ([], VpropList.tr_sub_of_ctx sb)).
+    - intros (s, sl) [b sb]%Sub.uncons.
+      exact (
+        let (r_vs, r_sb) := split_sub_of_ctx1 vs add sl sb in
+        (if b then r_vs else existT _ v s :: r_vs, r_sb)
+      ).
+  Defined.
+
+  Lemma split_sub_of_ctx1_sl vs add ncsm csm1 sl1i sl1a csm:
+    let sl1a' := VpropList.change_ctx_sub add csm1 sl1a in forall
+    (E : split_sub_of_ctx1 vs add (VpropList.app_sel sl1i sl1a') csm = (ncsm, csm1)),
+    SLprop.eq
+      (CTX.sl (CTX.sub (VpropList.inst (vs ++ VpropList.of_ctx add) (VpropList.app_sel sl1i sl1a'))
+                       (Sub.neg csm)))
+      (CTX.sl ncsm ** CTX.sl (CTX.sub add (Sub.neg csm1))).
+  Proof.
+    revert sl1i csm ncsm; induction vs as [|v vs]; cbn.
+    - intros _ ? ?.
+      injection 1 as <- E; SL.normalize.
+      induction add as [|[] add].
+      + reflexivity.
+      + destruct csm1 as [[|] csm1] using Sub.caseS';
+        cbn in sl1a.
+        * destruct sl1a as (sl0, sl1a); cbn in csm.
+          destruct csm as [b csm] using Sub.caseS'.
+          cbn in E; apply Vector.cons_inj in E as [-> E].
+          apply IHadd in E.
+          cbn; exact E.
+        * cbn in csm.
+          destruct csm as [b csm] using Sub.caseS'.
+          cbn in E; apply Vector.cons_inj in E as [-> E].
+          apply IHadd in E.
+          cbn; rewrite E; reflexivity.
+    - intros (sl, sl1i) csm ?.
+      case csm as [b csm] using Sub.caseS'; cbn.
+      specialize (IHvs sl1i csm); cbn in IHvs.
+      destruct split_sub_of_ctx1 as (r_vs, r_sb).
+      specialize (IHvs r_vs).
+      injection 1 as <- <-.
+      case b; cbn; rewrite IHvs by reflexivity;
+      SL.normalize; reflexivity.
+  Qed.
+
+  Let m (sel0 : VpropList.sel_t (vinv ini)) : CTX.t := VpropList.inst (vinv ini) sel0.
+
+  Section Loop_Spec1.
+    Variables (sel0 : VpropList.sel_t (vinv ini))
+              (add  : CTX.t)
+              (csm1 : Sub.t add).
+
+    Let vs1 (x : A + B) := vinv x ++ VpropList.of_ctx add.
+    Let vs2 (x : A + B) := vinv x ++ VpropList.of_ctx (CTX.sub add csm1).
+    Let RA  := TF.mk_p A (fun x => (vs1 (inl x))).
+    Let ctx1 (r : TF.t RA) := VpropList.inst (vs1 (inl (TF.v_val r))) (TF.v_sel r).
+
+    Definition r1_of_sub
+      (v : A)
+      (sl : TF.t (TF.p_tu (VpropList.sel (vinv (inl v) ++ VpropList.of_ctx (CTX.sub add csm1))))):
+      TF.t (TF.mk_p A (fun x => vinv (inl x) ++ VpropList.of_ctx add)).
+    Proof.
+      exists v.
+      apply TF.of_tu.
+      apply TF.to_tu, VpropList.split_sel in sl as (sl0, sl1).
+      exact (VpropList.app_sel sl0 (VpropList.change_ctx_sub add csm1 sl1)).
+    Defined.
+
+    Let s_f_t :=
+      TF.arrow RA (fun r1 => i_spec_t (A + B) (ctx1 r1)).
+    Let sel2_t (s_f : s_f_t) :=
+      TF.arrow RA (fun r1 => TF.arrow (sf_rvar (TF.to_fun s_f r1)) (fun r2 =>
+        VpropList.sel_t (vs2 (TF.v_val r2)))).
+
+    Let sel_0 :=
+      VpropList.app_sel sel0 (VpropList.sel_of_ctx (CTX.sub add csm1)).
+    Let ret_2 (s_f : s_f_t) (sel2 : sel2_t s_f) (r1 : TF.t RA) (r2 : sf_rvar_t (TF.to_fun s_f r1)):
+      TF.mk_t (A + B) vs2 :=
+      TF.mk _ (TF.v_val r2) (TF.to_fun (TF.to_fun sel2 r1) r2).
+      
+
+    Definition loop_sf_spec1 (s_f : s_f_t) (sel2 : sel2_t s_f)
+        (Inv : TF.arrow (TF.mk_p (A+B) vs2) (fun _ => Prop)):
+      FP.instr (TF.mk_p B (fun x : B => vs2 (inr x))) :=
+      @FunProg.Loop A B (fun x => TF.p_tu (VpropList.sel (vs2 x)))
+        Inv
+        ini (TF.of_tu sel_0)
+        (fun x : A => DTuple.of_fun (fun r1a =>
+         let r1 : TF.t RA := r1_of_sub x r1a in
+         FunProg.Bind (sf_spec (TF.to_fun s_f r1)) (TF.of_fun (fun r2 =>
+         FunProg.Ret (ret_2 s_f sel2 r1 r2))))).
+
+    Local Transparent FP.Bind FP.Ret FP.Loop.
+    Local Opaque ret_2 r1_of_sub TF.to_fun.
+
+    Lemma loop_sf_spec1_wlp s_f sel2 Inv post
+      (WLP : FP.wlp (loop_sf_spec1 s_f sel2 Inv) post):
+      TF.to_fun Inv (TF.mk _ ini sel_0) /\
+      (forall x1 sl1,
+        let r1 : TF.t RA := r1_of_sub x1 (TF.of_tu sl1) in
+        TF.to_fun Inv (TF.mk _ (inl x1) sl1) ->
+        FP.wlp (sf_spec (TF.to_fun s_f r1)) (fun r2 => TF.to_fun Inv (ret_2 s_f sel2 r1 r2))) /\
+      (forall x3 sl3,
+        TF.to_fun Inv (TF.mk _ (inr x3) sl3) ->
+        post (TF.mk _ x3 sl3)).
+    Proof.
+      cbn in WLP; case WLP as (INI & PRS & EXIT).
+      split; [|split].
+      - exact INI.
+      - intros x1 sl1 r1 INV1.
+        specialize (PRS x1 (TF.of_tu sl1) INV1).
+        rewrite TF.to_of_fun in PRS.
+        cbn in PRS; fold r1 in PRS.
+        eapply FP.wlp_monotone, PRS; cbn; intro r2.
+        rewrite DTuple.to_of_fun; cbn; auto.
+      - intros x3 sl3.
+        exact (EXIT x3 (TF.of_tu sl3)).
+    Qed.
+
+    Local Opaque loop_sf_spec1.
+    Local Transparent r1_of_sub.
+
+    Variable (EX :
+      forall (R : DTuple.p)
+             (f : forall Inv : TF.arrow (TF.mk_p (A + B) vs2) (fun _ => Prop),
+                  FP.instr R),
+      FP.instr R).
+
+    Inductive Loop_Spec1 : i_spec_t B (m sel0 ++ add) -> Prop
+      := Loop_Spec1I
+      (s_f    : s_f_t)
+      (S_F : TF.arrow RA (fun r =>
+        HasSpec CT (f (TF.v_val r)) (ctx1 r) (TF.to_fun s_f r)))
+      (sel2_f : sel2_t s_f)
+      (E : TF.arrow RA (fun r1 =>
+        let (ncsm, csm_add) :=
+          split_sub_of_ctx1 (vinv (inl (TF.v_val r1))) add
+                            (TF.v_sel r1) (sf_csm (TF.to_fun s_f r1)) in
+        csm1 = csm_add /\
+        TF.all (sf_rvar (TF.to_fun s_f r1)) (fun r2 => inhabited (
+          CTX.Trf.t (sf_prd_ctx (TF.to_fun s_f r1) r2 ++ ncsm)
+                    (VpropList.inst (vs2 (TF.v_val r2)) (TF.to_fun (TF.to_fun sel2_f r1) r2)))))):
+      Loop_Spec1 {|
+        sf_csm  := Sub.app (Sub.const (m sel0) true) csm1;
+        sf_prd  := fun x : B => vs2 (inr x);
+        sf_spec := EX _ (loop_sf_spec1 s_f sel2_f)
+      |}.
+
+    Lemma Loop_Spec1_correct
+      (EX_correct : forall R f post, FP.wlp (EX R f) post -> exists Inv, FP.wlp (f Inv) post)
+      s (SP : Loop_Spec1 s):
+      sound_spec CT (CP.Loop ini (fun x0 : A => i_impl (f x0))) (m sel0 ++ add) s.
+    Proof.
+      destruct SP; do 2 intro; cbn in post, PRE.
+      apply EX_correct in PRE as (Inv & (INI & PRS & EXIT)%loop_sf_spec1_wlp).
+      clear EX_correct.
+      pose (sl_inv := fun x : A + B =>
+        SLprop.ex (VpropList.sel_t (vs2 x)) (fun sl =>
+        SLprop.pure (TF.to_fun Inv (TF.mk _ x sl)) **
+        CTX.sl (VpropList.inst (vs2 x) sl) **
+        CTX.sl (CTX.sub add (Sub.neg csm1)))%slprop).
+
+      eapply SP.Cons. {
+        apply SP.Loop with (inv := sl_inv).
+        intro x1; unfold sl_inv.
+        apply SP.ExistsE; intro sl1.
+        apply SP.PureE;   intro INV1.
+        pose (r1  := r1_of_sub x1 (TF.of_tu sl1)).
+        apply TF.to_fun with (x := r1) in S_F, E.
+        eapply SP.Cons.
+          { apply S_F, PRS, INV1. }
+        clear S_F PRS INV1.
+
+        subst s_f_t sel2_t ret_2 ctx1; cbn beta in *.
+        set (r1'     := r1_of_sub _ _); change r1' with r1; clear r1'.
+        set (sel2_f1 := TF.to_fun sel2_f r1) in *; clearbody sel2_f1; clear sel2_f; cbn in sel2_f1.
+        set (s_f1    := TF.to_fun s_f r1) in *.
+          set (t := TF.to_fun _ _) in sel2_f1; change t with s_f1 in sel2_f1; clear t;
+          clearbody s_f1; clear s_f; cbn in s_f1.
+        unfold r1_of_sub in r1.
+        set (t := VpropList.split_sel _ _ _) in r1, s_f1, sel2_f1; subst r1.
+        set (t' := TF.to_tu _) in t;
+          assert (t' = sl1) by apply TF.to_of_tu;
+          clearbody t'; subst t'.
+        cbn in E.
+        specialize (VpropList.app_split_sel _ _ sl1) as sl1_eq;
+          fold t in sl1_eq; case t as [sl1i sl1a]; cbn in sl1_eq;
+          subst sl1.
+        cbn in E; cbn.
+        set (t := TF.to_tu _) in s_f1, E, sel2_f1; fold t.
+        eassert (t = _) by apply TF.to_of_tu; clearbody t; subst t.
+
+        split; unfold sf_post, sf_post_ctx; cbn.
+        - unfold vs1, vs2; cbn.
+          rewrite !VpropList.inst_app, !CTX.sl_app, VpropList.change_ctx_sub_sl.
+          SL.normalize; setoid_rewrite SLprop.star_comm at 2; reflexivity.
+        - intro x2; SL.normalize.
+          Intro sel2.
+          Intro POST.
+          pose (r2 := TF.mk (sf_prd s_f1) x2 sel2);
+            change (existT _ x2 (TF.of_tu sel2)) with r2.
+          Apply (TF.to_fun sel2_f1 r2).
+          Apply POST; clear POST.
+          subst vs1; cbn.
+          case split_sub_of_ctx1 as (ncsm, csm_add) eqn:E_eq in E;
+            case E as [<- E];
+            rewrite TF.all_iff in E; specialize (E r2);
+            case E as [E%CTX.Trf.t_fwd].
+          etransitivity.
+            2:apply SLprop.star_morph_imp; [exact E | reflexivity].
+          rewrite !CTX.sl_app; SL.normalize.
+          apply split_sub_of_ctx1_sl in E_eq as ->.
+          reflexivity.
+      }
+      clear E PRS.
+      split; unfold sf_post, sl_inv; cbn.
+      - unfold vs2, m.
+        Apply sel_0.
+        Apply INI.
+        unfold sel_0.
+        rewrite VpropList.inst_app, VpropList.inst_of_ctx, !CTX.sl_app,
+                (CTX.sl_split add csm1).
+        SL.normalize; reflexivity.
+      - intro x3.
+        unfold vs2, m, sl_inv.
+        Intro sel3. Intro INV3.
+        Apply sel3.
+        Apply. apply EXIT, INV3.
+        clear.
+        unfold Sub.neg, Sub.const.
+        rewrite TF.to_of_tu, CTX.sl_app, Sub.map_app, Vector.map_const,
+                Sub.sub_app, Sub.sub_const_false.
+        reflexivity.
+    Qed.
+  End Loop_Spec1.
+
+  Inductive Loop_Spec (ctx : CTX.t) (F : i_spec_t B ctx) : Prop
+    := Loop_SpecI
+    (sel0 : VpropList.sel_t (vinv ini))
+    (add  : CTX.t)
+    (csm1 : Sub.t add)
+    (s    : i_spec_t B (m sel0 ++ add))
+    (IJ   : InjPre_Spec (m sel0) ctx add s F)
+    (L1   : Loop_Spec1 sel0 add csm1 (fun R f =>
+              let isel (x : A + B) := VpropList.sel (vinv x ++ VpropList.of_ctx (CTX.sub add csm1)) in
+              match sinv with
+              | Some sinv =>
+                  f (fun (x : A + B) => TF.of_fun (T := TF.p_tu (isel x)) (fun sel =>
+                     let (seli, _) := VpropList.split_sel (vinv x) (VpropList.of_ctx (CTX.sub add csm1))
+                                        (DTuple.to_tu sel) in
+                     Tuple.to_fun (sinv x) seli))
+              | None =>
+                  FunProg.Bind
+                  (FunProg.Oracle (DTuple.Psingl
+                    (forall x : A + B, DTuple.arrow (DTuple.p_tu (isel x)) (fun _ => Prop))))
+                  f
+              end) s).
+  
+  Program Definition Loop0 : instr CT B := {|
+    i_impl := CP.Loop ini (fun x => i_impl (f x));
+    i_spec := fun ctx => Loop_Spec ctx;
+  |}.
+  Next Obligation.
+    destruct SP.
+    apply (Tr_InjPre  IJ); clear IJ.
+    eapply Loop_Spec1_correct, L1; clear;
+    intros R f post; case sinv as [|].
+    - intro H; eexists; exact H.
+    - intros [[Inv []] H]. exists Inv; exact H.
+  Qed.
+
+  Global Arguments loop_sf_spec1/.
+End Loop.
+Definition Loop [CT A B]
+  {inv : opt_arg (A + B -> list Vprop.t) (fun _ => [])}
+  (ini : A + B)
+  (body : A -> instr CT (A + B)):
+  instr CT B
+  := Loop0 inv None ini body.
+
+Definition Loop_inv [CT A B]
+  (inv : A + B -> {v : list Vprop.t & Tuple.arrow (VpropList.sel v) (fun _ => Prop)})
+  (ini : A + B)
+  (body : A -> instr CT (A + B)):
+  instr CT B
+  := Loop0 (fun x => projT1 (inv x)) (Some (fun x => projT2 (inv x))) ini body.
+
+Ltac build_Loop :=
+  simple refine (Loop_SpecI _ _ _ _ _ _ _ _ _ _ _ _);
+  [ (* sel0 *) cbn; Tuple.build_shape
+  | (* add  *) shelve | (* csm1 *) shelve | (* s    *) shelve
+  | (* IJ   *) Tac.build_InjPre
+  | (* L1   *)
+    simple refine (Loop_Spec1I _ _ _ _ _ _ _ _ _ _ _);
+    [ (* s_f    *) shelve
+    | (* S_F    *) cbn; intros; Tac.build_HasSpec
+    | (* sel2_f *) (* wait for csm1 *)
+    | (* E      *) cbn; intros; split; [reflexivity (* csm1 *)|] ];
+    [ (* sel2_f *) cbn; intros; Tuple.build_shape
+    | (* E      *) cbn; intros; constructor; CTX.Trf.Tac.build_t ]
+  ];
+  (* IJ spec eq *) Tac.cbn_refl.
+
 Module Tactics.
-  #[export] Hint Extern 1 (Read_Spec    _ _ _) => build_Read   : HasSpecDB.
-  #[export] Hint Extern 1 (Write_Spec _ _ _ _) => build_Write  : HasSpecDB.
+  #[export] Hint Extern 1 (Read_Spec       _ _ _) => build_Read   : HasSpecDB.
+  #[export] Hint Extern 1 (Write_Spec    _ _ _ _) => build_Write  : HasSpecDB.
+  #[export] Hint Extern 1 (Loop_Spec _ _ _ _ _ _) => build_Loop   : HasSpecDB.
 End Tactics.
 Export Tactics.
